modularized weakening

FOL.v
@@ -1,6 +1,8 @@
 Require Export syntax.
 
 Reserved Notation "A ⊢ p" (at level 70).
+Reserved Notation "A ⊢I p" (at level 70).
+Reserved Notation "A ⊢U p" (at level 70).
 
 Notation "p ~> q" := (Impl_ _ _ p q) (at level 60).
 Notation "⊥" := (Fal_ _ _).
@@ -19,29 +21,32 @@ Section implicative.
     | Impl _ p q => count p + count q
   end.
 
-  Inductive nd_imp (A : list form) : form -> Prop :=
-    | ndHI p : In p A -> A ⊢ p
-    | ndExp p : A ⊢ ⊥ -> A ⊢ p
-    | ndII p q : (p :: A) ⊢ q -> A ⊢ p ~> q
-    | ndIE p q : A ⊢ p ~> q -> A ⊢ p -> A ⊢ q
-  where "A ⊢ p" := (nd_imp A p).
 
   Variable nd : list form -> form -> Prop.
+  Notation "A ⊢ p" := (nd A p) (at level 70).
+  Inductive nd_imp (A : list form) : form -> Prop :=
+    | ndHI p : In p A -> A ⊢I p
+    | ndExp p : A ⊢ ⊥ -> A ⊢I p
+    | ndII p q : (p :: A) ⊢ q -> A ⊢I p ~> q
+    | ndIE p q : A ⊢ p ~> q -> A ⊢ p -> A ⊢I q
+  where "A ⊢I p" := (nd_imp A p).
+  Variable agree : forall A p, nd A p -> A ⊢I p.
 
-  Lemma weakening_imp A B p : A ⊢ p -> incl A B -> B ⊢ p.
+  Variable weakening : forall A B p, A ⊢ p -> incl A B -> B ⊢ p.
+  Lemma weakening_imp A B p : A ⊢I p -> incl A B -> B ⊢I p.
   Proof. intro. revert B. induction H; intros B Hinc.
     -apply ndHI. now apply Hinc.
-    -apply ndExp. now apply IHnd_imp.
-    -apply ndII, (IHnd_imp (p::B)). { apply incl_cons. now left. now apply incl_tl. }
-    -apply (ndIE _ p). now apply IHnd_imp1. now apply IHnd_imp2.
+    -apply ndExp. now apply (weakening A).
+    -apply ndII. apply (weakening (p::A) (p::B)). assumption. { apply incl_cons. now left. now apply incl_tl. }
+    -apply (ndIE _ p). now apply (weakening A B (p~>q)). now apply (weakening A).
   Qed.
 
-  Lemma double_neg_imp A p : A ⊢ p -> A ⊢ ¬¬p.
+(*   Lemma double_neg_imp A p : A ⊢ p -> A ⊢ ¬¬p.
   Proof. apply (ndIE _ p), ndII, ndII. apply (ndIE _ p).
     { apply ndHI. now left. }
     { apply ndHI. right. now left. }
   Qed.
-
+ *)
 End implicative.
 
 Section universals.
@@ -57,24 +62,26 @@ Section universals.
   end.
 
   Variable nd : list form -> form -> Prop.
-
+  Notation "A ⊢ p" := (nd A p) (at level 70).
   Definition up_ctx (A : list form) := map (subst_form (S >> var_term)) A.
   Inductive nd_univ (A : list form) : form -> Prop :=
-    | ndUI p : up_ctx A ⊢ p -> A ⊢ ∀ p
-    | ndUE p t : A ⊢ ∀ p -> A ⊢ subst_form (t ..) p
-  where "A ⊢ p" := (nd_univ A p).
+    | ndUI p : up_ctx A ⊢ p -> A ⊢U ∀ p
+    | ndUE p t : A ⊢ ∀ p -> A ⊢U subst_form (t ..) p
+  where "A ⊢U p" := (nd_univ A p).
 
-  Lemma weakening_univ A B p : A ⊢ p -> incl A B -> B ⊢ p.
+
+  Variable weakening : forall A B p, A ⊢ p -> incl A B -> B ⊢ p.
+  Lemma weakening_univ A B p : A ⊢U p -> incl A B -> B ⊢U p.
   Proof. intro. revert B. induction H; intros B Hinc.
-    -apply ndUI, (IHnd_univ (up_ctx B)). unfold up_ctx. now apply incl_map.
-    -apply ndUE. now apply IHnd_univ.
+    -apply ndUI. apply (weakening (up_ctx A) (up_ctx B)). assumption. unfold up_ctx. now apply incl_map.
+    -apply ndUE. now apply (weakening A).
   Qed.
 
-  Variable retract_implicative : retract (form_implicative form) form.
+ (*  Variable retract_implicative : retract (form_implicative form) form.
   Variable equiv_nd : forall A p, nd_imp _ _ A p <-> nd_univ A p.
   Lemma double_neg_univ A (p : form) : A ⊢ p -> A ⊢ ¬¬( p).
   Proof. intro. apply equiv_nd. apply (double_neg_imp _ _ A (p)). now apply equiv_nd.
-  Qed.
+  Qed. *)
 
 End universals.
 
@@ -83,20 +90,14 @@ Fixpoint count (p : form) := match p with
   | In_form_univ p => count_univ _ count p
 end.
 
-Definition nd (A : list form) (p : form) : Prop := match p with
-  | In_form_implicative _ => nd_imp _ _ A p
-  | In_form_univ _ => nd_univ _ _ subst_form A p
-end.
-Notation "A ⊢ p" := (nd A p) (at level 70).
+Inductive nd : list form -> form -> Prop := 
+  | ndI A p : nd_imp form _ nd A p -> A ⊢ p
+  | ndU A p : nd_univ form _ subst_form nd A p -> A ⊢ p
+where "A ⊢ p" := (nd A p).
 
-Lemma weakening A B p : A ⊢ p -> incl A B -> B ⊢ p.
-Proof. destruct p.
-  -apply weakening_imp.
-  -apply weakening_univ.
+Fixpoint weakening A B p: A ⊢ p -> incl A B -> B ⊢ p.
+Proof. destruct 1; intro Hinc.
+    -apply ndI. now apply (weakening_imp _ _ nd weakening A B).
+    -apply ndU. now apply (weakening_univ _ _ subst_form nd weakening A B).
 Qed.
 
-Lemma double_neg A p : A ⊢ p -> A ⊢ ¬¬p.
-Proof. destruct p.
-  -apply double_neg_imp.
-  -Check double_neg_univ.
-Admitted.
